realsum.bpl
@@ -1,4 +1,6 @@
 type Ref;
+var packedBasicFieldsRealSum: [Ref] bool;
+var fracBasicFieldsRealSum: [Ref] real;
 var packedSumOKRealSum: [Ref] bool;
 var fracSumOKRealSum: [Ref] real;
 var packedSumGreater0RealSum: [Ref] bool;
@@ -8,6 +10,14 @@ const null: Ref;
 
 var n: [Ref]int;
 var sum: [Ref]real;
+
+procedure PackBasicFieldsRealSum(s1:real, n1:int, this:Ref);
+requires (packedBasicFieldsRealSum[this] == false);
+requires (sum[this] == s1) && (n[this]==n1);
+
+procedure UnpackBasicFieldsRealSum(s1:real, n1:int, this:Ref);
+requires packedBasicFieldsRealSum[this];
+ensures (sum[this] == s1) && (n[this]==n1);
 
 procedure PackSumOKRealSum(s1:real, n1:int, this:Ref);
 requires (packedSumOKRealSum[this] == false);
@@ -27,16 +37,9 @@ procedure UnpackSumGreater0RealSum(s1:real, this:Ref);
 requires packedSumGreater0RealSum[this];
 ensures (sum[this] == s1) && (s1 > 0.0);
 
-procedure ConstructRealSum(this:Ref);
-ensures n[this] == 0;
-ensures sum[this] == 0;
-
-procedure sumConstrRealSum(n1:int, this:Ref)
-modifies n, sum;
-{
-n[this]:=n1;
-call calculateRealSum(n[this], this);
-}
+procedure ConstructRealSum(n1:int, s:Ref, this:Ref);
+ensures n[this] == n1;
+ensures sum[this] == s;
 
 procedure calculateRealSum(n1: int, this:Ref) 
 modifies sum;
@@ -44,10 +47,14 @@ modifies sum;
 	sum[this] := n1 * (n1 + 1) / 2;
 }
 
-procedure calculateSumRealSum(this:Ref)  returns (r:real)
+procedure calculateSumRealSum(n1:int, this:Ref)  returns (r:real)
+modifies n, sum;
+requires packedBasicFieldsRealSum[this] && fracBasicFieldsRealSum[this]==1.0
+ensures packedSumOKRealSum[this] && fracSumOKRealSum[this]==1.0
 
 { 
-	r:= sum[this];
+        n[this]:=n1;
+	call r:= calculateRealSum(n1, this);
 }
 
 procedure sumIsOKRealSum( this:Ref) returns (r:bool) {
